coq/HyperLedgerComposerQuery/Lang/HLCQuerySemEval.v
@@ -1,0 +1,296 @@
+(*
+ * Copyright 2015-2016 IBM Corporation
+ *
+ * Licensed under the Apache License, Version 2.0 (the "License");
+ * you may not use this file except in compliance with the License.
+ * You may obtain a copy of the License at
+ *
+ * http://www.apache.org/licenses/LICENSE-2.0
+ *
+ * Unless required by applicable law or agreed to in writing, software
+ * distributed under the License is distributed on an "AS IS" BASIS,
+ * WITHOUT WARRANTIES OR CONDITIONS OF ANY KIND, either express or implied.
+ * See the License for the specific language governing permissions and
+ * limitations under the License.
+ *)
+
+Section HLCQuerySemantics.
+  Require Import String.
+  Require Import List.
+  Require Import Arith.
+  Require Import EquivDec.
+  Require Import Utils.
+  Require Import CommonRuntime.
+
+  Require Import HLCQueryDef.
+  Require Import HLCQueryDec.
+  Require Import HLCQuerySemantics.
+  Require Import HLCQueryEval.  
+  Context {fruntime:foreign_runtime}.
+
+  (* Proof that the semantic relation and evaluation function are the same *)
+
+  Context (h:brand_relation_t).
+  Section correctness.
+
+    (*  Move to Utils, somewhere appropriate *)
+    Lemma some_olift {A B} {f:A->option B} {x} {y} :
+      olift f x = Some y -> {z : A | x = Some z & Some y = f z}.
+    Proof.
+      unfold olift.
+      destruct x; try discriminate.
+      eauto.
+    Qed.
+
+    Lemma some_olift2 {A B C} {f:A->B->option C} {x} {y} {z} :
+      olift2 f x y = Some z -> {x' : A & {y':B | x = Some x' /\ y = Some y' & Some z = f x' y'}}.
+    Proof.
+      unfold olift2.
+      destruct x; try discriminate.
+      destruct y; try discriminate.
+      eauto.
+    Qed.
+
+    Lemma some_lift2 {A B C} {f:A->B->C} {x} {y} {z} :
+      lift2 f x y = Some z -> {x' : A & {y':B | x = Some x' /\ y = Some y' & z = f x' y'}}.
+    Proof.
+      unfold lift2.
+      destruct x; try discriminate.
+      destruct y; try discriminate.
+      inversion 1; eauto.
+    Qed.
+
+    Lemma hlcquery_statement_from_sem_eval_same reg_name registries res :
+      hlcquery_statement_from_sem reg_name registries res <->
+      hlcquery_statement_from_eval (with_default reg_name "default"%string) registries = Some res.
+    Proof.
+      unfold hlcquery_statement_from_eval, with_default.
+      split; intros.
+      - invcs H; trivial.
+      - match_destr_in H; constructor; trivial.
+    Qed.
+
+    Lemma hlcquery_statement_select_sem_eval_same b dl res :
+      hlcquery_statement_select_sem h b dl res <->
+      hlcquery_statement_select_eval h b dl = Some res.
+    Proof.
+      split; revert b res.
+      - { induction dl; simpl in *; intros; inversion H; simpl; subst.
+          - reflexivity.
+          - rewrite hlcquery_statement_select_eval_cons_subrec; trivial.
+            erewrite IHdl; eauto.
+            reflexivity.
+          - rewrite hlcquery_statement_select_eval_cons_nsub; trivial.
+            erewrite IHdl; eauto.
+        }
+      - { induction dl; simpl in *; intros.
+          - inversion H; subst; constructor.
+          - destruct a; try solve [inversion H].
+            destruct (sub_brands_dec h b0 (singleton b)) as [sub|nsub].
+            + destruct (hlcquery_statement_select_eval_cons_sub_some_rec h sub H)
+              ; subst.
+              rewrite hlcquery_statement_select_eval_cons_subrec in H by trivial.
+              apply some_lift in H; destruct H as [? ? ?]; subst.
+              apply hlcquery_statement_select_sem_cons; auto.
+            + rewrite hlcquery_statement_select_eval_cons_nsub in H by trivial.
+              apply hlcquery_statement_select_sem_skip; auto.
+        }
+    Qed.
+
+    Lemma hlcquery_condition_expr_sem_eval_same c params fields res :
+      hlcquery_condition_expr_sem h c params fields res <->
+      hlcquery_condition_expr_eval h c params fields = Some res.
+    Proof.
+      split; revert params fields res.
+      - { induction c; simpl in *; intros; inversion H; simpl; subst; try eauto 3.
+          - apply IHc in H2; rewrite H2; simpl; trivial.
+          - apply IHc1 in H3; rewrite H3.
+            apply IHc2 in H7; rewrite H7.
+            simpl; trivial.
+        }            
+      - { induction c; simpl in *; intros.
+          - inversion H; subst; constructor.
+          - constructor; trivial.
+          - constructor; trivial.
+          - apply some_olift in H; destruct H as [? ev1 ?].
+            apply IHc in ev1.
+            econstructor; eauto.
+          - apply some_olift2 in H; destruct H as [? [? [ev1 ev2] ?]].
+            apply IHc1 in ev1.
+            apply IHc2 in ev2.
+            econstructor; eauto.
+        }
+    Qed.
+
+    Lemma hlcquery_condition_sem_eval_same c params fields res :
+      hlcquery_condition_sem h c params fields res <->
+      hlcquery_condition_eval h c params fields = Some res.
+    Proof.
+      split; revert params fields res.
+      - { induction c; simpl in *; intros; inversion H; simpl; subst.
+          - apply IHc1 in H2; rewrite H2.
+            apply IHc2  in H6; rewrite H6.
+            simpl; trivial.
+          - apply IHc1 in H2; rewrite H2.
+            apply IHc2  in H6; rewrite H6.
+            simpl; trivial.
+          - apply hlcquery_condition_expr_sem_eval_same in H2; rewrite H2.
+            apply hlcquery_condition_expr_sem_eval_same in H3; rewrite H3.
+            simpl.
+            destruct (in_dec data_eq_dec d l); tauto.
+          - apply hlcquery_condition_expr_sem_eval_same in H2; rewrite H2.
+            apply hlcquery_condition_expr_sem_eval_same in H3; rewrite H3.
+            simpl.
+            destruct (in_dec data_eq_dec d l); tauto.
+          - apply hlcquery_condition_expr_sem_eval_same in H1; rewrite H1.
+            trivial.
+        }            
+      - { induction c; simpl in *; intros.
+          - apply some_olift2 in H; destruct H as [? [? [ev1 ev2] ?]].
+            invcs e.
+            constructor; eauto.
+          - apply some_olift2 in H; destruct H as [? [? [ev1 ev2] ?]].
+            invcs e.
+            constructor; eauto.
+          - match_case_in H; [intros ? eq1 | intros eq1]; rewrite eq1 in H; try discriminate.
+            destruct d; try discriminate.
+            invcs H.
+            apply some_olift2 in eq1; destruct eq1 as [? [? [ev1 ev2] ?]].
+            apply hlcquery_condition_expr_sem_eval_same in ev1.
+            apply hlcquery_condition_expr_sem_eval_same in ev2.
+            simpl in e.
+            unfold ondcoll in e.
+            destruct x0; try discriminate.
+            invcs e.
+            match_destr_in H0; invcs H0; econstructor; eauto.
+          - match_case_in H; [intros ? eq1 | intros eq1]; rewrite eq1 in H; try discriminate.
+            destruct d; try discriminate.
+            invcs H.
+            apply hlcquery_condition_expr_sem_eval_same in eq1.
+            constructor; eauto.
+        }
+    Qed.
+
+    Lemma hlcquery_condition_filter_sem_eval_same c params dl res :
+      hlcquery_condition_filter_sem h c params dl res <->
+      hlcquery_condition_filter_eval h c params dl = Some res.
+    Proof.
+      split; revert c params res.
+      - { induction dl; simpl in *; intros; simpl; invcs H.
+          - reflexivity.
+          - apply hlcquery_condition_sem_eval_same in H4; rewrite H4.
+            erewrite IHdl; eauto; reflexivity.
+          - apply hlcquery_condition_sem_eval_same in H4; rewrite H4.
+            erewrite IHdl; eauto; reflexivity.
+        } 
+      - { induction dl; simpl in *; intros.
+          - invcs H; constructor.
+          - apply some_lift2 in H; destruct H as [? [? [ev1 ev2] ?]].
+            apply hlcquery_condition_sem_eval_same in ev1.
+            apply IHdl in ev2.
+            destruct x; subst; econstructor; eauto.
+        }
+    Qed.
+
+    Lemma hlcquery_condition_filter_optional_sem_eval_same cond params dl res :
+      hlcquery_condition_filter_optional_sem h cond params dl res <->
+      (match cond with
+                            | Some c => hlcquery_condition_filter_eval h c params dl
+                            | None => Some dl
+                            end) = Some res.
+    Proof.
+      split; intros.
+      - invcs H; trivial.
+        apply hlcquery_condition_filter_sem_eval_same; trivial.
+      - destruct cond.
+        + constructor.
+          apply hlcquery_condition_filter_sem_eval_same; trivial.
+        + invcs H.
+          constructor.
+    Qed.
+    
+    Lemma hlcquery_statement_order_sem_eval_same ord dl res :
+      hlcquery_statement_order_sem ord dl res <->
+      apply_optional (lift hlcquery_statement_order_eval ord) dl = res.
+    Proof.
+      unfold hlcquery_statement_order_eval, apply_optional, with_default.
+      split; intros.
+      - invcs H.
+        destruct ord; simpl; reflexivity.
+      - destruct ord; simpl in *; subst; constructor.
+    Qed.
+
+    Lemma hlcquery_statement_skip_sem_eval_same skip dl res :
+      hlcquery_statement_skip_sem skip dl res <->
+      apply_optional (lift hlcquery_statement_skip_eval skip) dl = res.
+    Proof.
+      unfold hlcquery_statement_skip_eval.
+      split; intros.
+      - destruct skip; simpl; invcs H; trivial.
+      - destruct skip; simpl in *; subst; constructor.
+    Qed.
+
+    Lemma hlcquery_statement_limit_sem_eval_same limit dl res :
+      hlcquery_statement_limit_sem limit dl res <->
+      apply_optional (lift hlcquery_statement_limit_eval limit) dl = res.
+    Proof.
+      unfold hlcquery_statement_limit_eval.
+      split; intros.
+      - destruct limit; simpl; invcs H; trivial.
+      - destruct limit; simpl in *; subst; constructor.
+    Qed.
+    
+    Lemma hlcquery_statement_sem_eval_same stmt registries params res :
+      hlcquery_statement_sem h stmt registries params res <->
+      hlcquery_statement_eval h stmt registries params = Some res.
+    Proof.
+      unfold hlcquery_statement_eval.
+      destruct stmt.
+      split; intros.
+      - invcs H.
+        apply hlcquery_statement_from_sem_eval_same in H6; rewrite H6; simpl.
+        apply hlcquery_statement_select_sem_eval_same in H10; rewrite H10; simpl.
+        apply hlcquery_condition_filter_optional_sem_eval_same in H11; rewrite H11; simpl.
+        apply hlcquery_statement_order_sem_eval_same in H12; rewrite H12; simpl.
+        apply hlcquery_statement_skip_sem_eval_same in H13; rewrite H13; simpl.
+        apply hlcquery_statement_limit_sem_eval_same in H14; rewrite H14; simpl.
+        trivial.
+      - unfold bind in H.
+        apply some_olift in H.
+        destruct H as [? from rest].
+        apply hlcquery_statement_from_sem_eval_same in from.
+        symmetry in rest.
+        apply some_olift in rest.
+        destruct rest as [? sel rest].
+        apply hlcquery_statement_select_sem_eval_same in sel.
+        symmetry in rest.
+        apply some_olift in rest.
+        destruct rest as [? filter rest].
+        apply hlcquery_condition_filter_optional_sem_eval_same in filter.
+        invcs rest.
+        eapply hlcquery_statement_sem_holds; eauto.
+        + eapply hlcquery_statement_order_sem_eval_same;  eauto.
+        + eapply hlcquery_statement_skip_sem_eval_same; eauto.
+        + eapply hlcquery_statement_limit_sem_eval_same; eauto.
+    Qed.
+
+    Theorem hlcquery_sem_eval_same q registries params res :
+      hlcquery_sem h q registries params res <->
+      hlcquery_eval h q registries params = Some res.
+    Proof.
+      unfold hlcquery_eval; simpl.
+      split; intros.
+      - invcs H; simpl.
+        apply hlcquery_statement_sem_eval_same; trivial.
+      - destruct q; constructor; apply hlcquery_statement_sem_eval_same; trivial.
+    Qed.
+
+  End correctness.
+
+End HLCQuerySemantics.
+
+(* 
+*** Local Variables: ***
+*** coq-load-path: (("../../../coq" "Qcert")) ***
+*** End: ***
+*)
