coq/HyperLedgerComposerQuery/Lang/HLCQuerySemantics.v
@@ -1,0 +1,219 @@
+(*
+ * Copyright 2015-2016 IBM Corporation
+ *
+ * Licensed under the Apache License, Version 2.0 (the "License");
+ * you may not use this file except in compliance with the License.
+ * You may obtain a copy of the License at
+ *
+ * http://www.apache.org/licenses/LICENSE-2.0
+ *
+ * Unless required by applicable law or agreed to in writing, software
+ * distributed under the License is distributed on an "AS IS" BASIS,
+ * WITHOUT WARRANTIES OR CONDITIONS OF ANY KIND, either express or implied.
+ * See the License for the specific language governing permissions and
+ * limitations under the License.
+ *)
+
+Section HLCQuerySemantics.
+  Require Import String.
+  Require Import List.
+  Require Import Arith.
+  Require Import EquivDec.
+  Require Import Utils.
+  Require Import CommonRuntime.
+
+  Require Import HLCQueryDef.
+  Require Import HLCQueryDec.
+  
+  Context {fruntime:foreign_runtime}.
+
+  (** Semantics for HLCQuery *)
+
+  Context (h:brand_relation_t).
+  Section sem.
+
+    Inductive hlcquery_statement_from_sem :
+      option registry_name ->
+      list (registry_name*(list data)) ->
+      list data ->
+      Prop :=
+    | hlcquery_statement_from_sem_default registries reg :
+        lookup string_dec registries "default"%string = Some reg ->
+        hlcquery_statement_from_sem None registries reg
+    | hlcquery_statement_from_sem_some registries regname reg :
+        lookup string_dec registries regname = Some reg ->
+        hlcquery_statement_from_sem (Some regname) registries reg.
+
+    Inductive hlcquery_statement_select_sem :
+              brand -> list data -> list (hlcquery_datum) -> Prop
+      :=
+      | hlcquery_statement_select_sem_nil b :
+           hlcquery_statement_select_sem b nil nil
+      | hlcquery_statement_select_sem_cons b b' r dl res :
+          sub_brands h b' (singleton b) ->
+          hlcquery_statement_select_sem b dl res ->
+          hlcquery_statement_select_sem b (dbrand b' (drec r)::dl) (r::res)
+      | hlcquery_statement_select_sem_skip b b' d dl res :
+          ~ sub_brands h b' (singleton b) ->
+          hlcquery_statement_select_sem b dl res ->
+          hlcquery_statement_select_sem b (dbrand b' d::dl) res.
+
+    Inductive hlcquery_condition_expr_sem
+      : hlcquery_condition_expr ->
+        list (string*data) ->
+        list (string*data) ->
+        data ->
+        Prop :=
+    | hlcquery_condition_expr_sem_const d params fields:
+        hlcquery_condition_expr_sem (hlcquery_condition_expr_const d) params fields d
+    | hlcquery_condition_expr_sem_param p params fields d:
+        lookup string_dec params p = Some d ->
+        hlcquery_condition_expr_sem (hlcquery_condition_expr_param p) params fields d
+    | hlcquery_condition_expr_sem_var v params fields d:
+        lookup string_dec fields v = Some d ->
+        hlcquery_condition_expr_sem (hlcquery_condition_expr_var v) params fields d
+    | hlcquery_condition_expr_sem_unop u c1 d1 params fields d:
+        hlcquery_condition_expr_sem c1 params fields d1 ->
+        unary_op_eval h u d1 = Some d ->
+        hlcquery_condition_expr_sem (hlcquery_condition_expr_unop u c1) params fields d
+    | hlcquery_condition_expr_sem_binop b c1 d1 c2 d2 params fields d:
+        hlcquery_condition_expr_sem c1 params fields d1 ->
+        hlcquery_condition_expr_sem c2 params fields d2 ->
+        binary_op_eval h b d1 d2 = Some d ->
+        hlcquery_condition_expr_sem (hlcquery_condition_expr_binop b c1 c2) params fields d
+    .
+    
+    Inductive hlcquery_condition_sem :
+      hlcquery_condition ->
+      list (string*data) ->
+      list (string*data) ->
+      bool ->
+      Prop :=
+    | hlcquery_condition_sem_and c1 c2 params fields b1 b2 :
+        hlcquery_condition_sem c1 params fields b1 ->
+        hlcquery_condition_sem c2 params fields b2 ->
+        hlcquery_condition_sem (hlcquery_condition_and c1 c2) params fields (andb b1 b2)
+    | hlcquery_condition_sem_or c1 c2 params fields b1 b2 :
+        hlcquery_condition_sem c1 params fields b1 ->
+        hlcquery_condition_sem c2 params fields b2 ->
+        hlcquery_condition_sem (hlcquery_condition_or c1 c2) params fields (orb b1 b2)
+    | hlcquery_condition_sem_contains_true ce1 ce2 params fields d l :
+        hlcquery_condition_expr_sem ce1 params fields d ->
+        hlcquery_condition_expr_sem ce2 params fields (dcoll l) ->
+        In d l ->
+        hlcquery_condition_sem (hlcquery_condition_contains ce1 ce2) params fields true
+    | hlcquery_condition_sem_contains_false ce1 ce2 params fields d l :
+        hlcquery_condition_expr_sem ce1 params fields d ->
+        hlcquery_condition_expr_sem ce2 params fields (dcoll l) ->
+        ~ In d l ->
+        hlcquery_condition_sem (hlcquery_condition_contains ce1 ce2) params fields false
+    | hlcquery_condition_sem_lifted ce params fields b  :
+        hlcquery_condition_expr_sem ce params fields (dbool b) ->
+        hlcquery_condition_sem (hlcquery_condition_lifted_expr ce) params fields b
+    .
+
+    Inductive hlcquery_condition_filter_sem :
+      hlcquery_condition ->
+      list (string*data) ->
+      list hlcquery_datum ->
+      list hlcquery_datum ->
+      Prop
+      :=
+      | hlcquery_condition_filter_sem_nil cond params:
+           hlcquery_condition_filter_sem cond params nil nil
+      | hlcquery_condition_filter_sem_cons cond params d dl res :
+          hlcquery_condition_sem cond params d true ->
+          hlcquery_condition_filter_sem cond params dl res ->
+          hlcquery_condition_filter_sem cond params (d::dl) (d::res)
+      | hlcquery_condition_filter_sem_skip cond params d dl res :
+          hlcquery_condition_sem cond params d false ->
+          hlcquery_condition_filter_sem cond params dl res ->
+          hlcquery_condition_filter_sem cond params (d::dl) res.
+
+    Inductive hlcquery_condition_filter_optional_sem :
+      option (hlcquery_condition) ->
+      list (string*data) ->
+      list hlcquery_datum ->
+      list hlcquery_datum ->
+      Prop :=
+      | hlcquery_condition_filter_optional_sem_none params dl :
+           hlcquery_condition_filter_optional_sem None params dl dl
+      |  hlcquery_condition_filter_optional_sem_some c params dl res :
+         hlcquery_condition_filter_sem c params dl res ->
+         hlcquery_condition_filter_optional_sem (Some c) params dl res
+    .
+    
+    Definition hlcquery_statement_order_sem (order:option hlcquery_ordering) (dl:list hlcquery_datum) (res:list hlcquery_datum)
+      := dl = res.
+
+    Inductive hlcquery_statement_skip_sem :
+      option nat ->
+      list hlcquery_datum ->
+      list hlcquery_datum ->
+      Prop :=
+    |  hlcquery_statement_skip_sem_none dl :
+         hlcquery_statement_skip_sem None dl dl
+    |  hlcquery_statement_skip_sem_some skip dl :
+         hlcquery_statement_skip_sem (Some skip) dl (skipn skip dl)
+    .
+
+    Inductive hlcquery_statement_limit_sem :
+      option nat ->
+      list hlcquery_datum ->
+      list hlcquery_datum ->
+      Prop :=
+    |  hlcquery_statement_limit_sem_none dl :
+         hlcquery_statement_limit_sem None dl dl
+    |  hlcquery_statement_limit_sem_some limit dl :
+         hlcquery_statement_limit_sem (Some limit) dl (firstn limit dl)
+    .
+
+    Inductive hlcquery_statement_sem :
+      hlcquery_statement ->
+      list (registry_name*(list data)) ->
+      list (string*data) ->
+      list hlcquery_datum ->
+      Prop :=
+    | hlcquery_statement_sem_holds
+        select_brand reg_name cond ordering skip limit
+        registries params
+        regdata
+        selected
+        filtered
+        ordered
+        skipped
+        result
+      :
+        hlcquery_statement_from_sem reg_name registries regdata ->
+        hlcquery_statement_select_sem select_brand regdata selected ->
+        hlcquery_condition_filter_optional_sem cond params selected filtered ->
+        hlcquery_statement_order_sem ordering filtered ordered ->
+        hlcquery_statement_skip_sem skip ordered skipped ->
+        hlcquery_statement_limit_sem limit skipped result ->
+          hlcquery_statement_sem
+          (mk_hlcquery_statement select_brand reg_name cond ordering skip limit)
+          registries
+          params
+          result.
+
+    Inductive hlcquery_sem :
+      hlcquery ->
+      list (registry_name*(list data)) ->
+      list (string*data) ->
+      list hlcquery_datum ->
+      Prop := 
+    | hlcquery_sem_holds
+        name desc stmt
+        registries params res :
+        hlcquery_statement_sem stmt registries params res ->
+        hlcquery_sem (mk_hlcquery name desc stmt) registries params res.
+
+  End sem.
+
+End HLCQuerySemantics.
+
+(* 
+*** Local Variables: ***
+*** coq-load-path: (("../../../coq" "Qcert")) ***
+*** End: ***
+*)
